Reduction

code/experimental/P256/Hacl.Impl.SolinasReduction.fst
@@ -98,19 +98,21 @@ let upl_fir_buffer c11 c12 c13 c14 c15 temp o =
 
 
 val upl_sec_buffer: c12: uint32 -> c13: uint32 -> c14: uint32 -> c15: uint32 
+  -> temp: lbuffer uint64 (size 4) 
   -> o: lbuffer uint64 (size 4) -> 
   Stack unit
     (requires fun h -> live h o )
-    (ensures fun h0 _ h1 -> modifies1 o h0 h1 /\
+    (ensures fun h0 _ h1 -> modifies2 o temp h0 h1 /\
       (
       	let o = as_seq h1 o in felem_seq_as_nat o == 
 	     (uint_v c12 * pow2 (3 * 32) + uint_v c13 * pow2 (4 * 32) + 
-        uint_v c14 * pow2 (5 * 32) + uint_v c15 * pow2 (6 * 32)) % prime
+        uint_v c14 * pow2 (5 * 32) + uint_v c15 * pow2 (6 * 32)) % prime /\
+	felem_seq_as_nat o < prime
       )
  )
 
 
-let upl_sec_buffer c12 c13 c14 c15 o = 
+let upl_sec_buffer c12 c13 c14 c15 temp o = 
   assert_norm (pow2 (1 * 32) * pow2 (2 * 32) = pow2 (3 * 32));
   assert_norm (pow2 (2 * 32) * pow2 (2 * 32) = pow2 (4 * 32));
   assert_norm (pow2 (3 * 32) * pow2 (2 * 32) = pow2 (5 * 32));
@@ -306,6 +308,118 @@ let upl_eig_buffer c9 c10 c11 c12 c13 c14 c15 temp o =
     reduction_prime_2prime_impl temp o
 
 
+val solinas_reduction_mod: 
+  c0_n: _uint32-> 
+  c1_n: _uint32 -> 
+  c2_n: _uint32 -> 
+  c3_n: _uint32 -> 
+  c4_n: _uint32 -> 
+  c5_n: _uint32 -> 
+  c6_n: _uint32 -> 
+  c7_n: _uint32 -> 
+  c8_n: _uint32 -> 
+  c9_n: _uint32 -> 
+  c10_n: _uint32 -> 
+  c11_n: _uint32 -> 
+  c12_n: _uint32 -> 
+  c13_n: _uint32 -> 
+  c14_n: _uint32 -> 
+  c15_n: _uint32->
+  s0: int {s0 = (c0_n + c1_n * pow2 32 + c2_n * pow2 (2 * 32) + c3_n * pow2 (3 * 32) + c4_n * pow2 (4 * 32) + c5_n * pow2 (5 * 32) + c6_n * pow2 (6 * 32) + c7_n * pow2 (7 * 32)) % prime} -> 
+  s1: int {s1 = (c11_n * pow2 (3 * 32) + c12_n * pow2 (4 * 32) + c13_n * pow2 (5 * 32) + c14_n * pow2 (6 * 32) + c15_n * pow2 (7 * 32)) % prime} ->
+  s2: int {s2 = (c12_n * pow2 (3 * 32) + c13_n * pow2 (4 * 32) + c14_n * pow2 (5* 32) + c15_n * pow2 (6 * 32)) % prime} -> 
+  s3: int {s3 = (c8_n + c9_n * pow2 32 + c10_n * pow2 (2 * 32) + c14_n * pow2 (6 * 32) + c15_n * pow2 (7 * 32)) % prime} ->
+  s4: int {s4 = (c9_n + c10_n * pow2 32 + c11_n * pow2 (2 * 32) + c13_n * pow2 (3 * 32) + c14_n * pow2 (4 * 32) + c15_n * pow2 (5 * 32) + c13_n * pow2 (6 * 32) + c8_n * pow2 (7 * 32)) % prime} -> 
+  s5: int {s5 = (c11_n + c12_n * pow2 32 + c13_n * pow2 (2 * 32) + c8_n * pow2 (6 * 32) + c10_n * pow2 (7 * 32)) % prime} ->
+  s6: int {s6 = (c12_n + c13_n * pow2 32 + c14_n * pow2 (2 * 32) + c15_n * pow2 (3 * 32) + c9_n * pow2 (6 * 32) + c11_n * pow2 (7 * 32)) % prime} ->
+  s7: int {s7 = (c13_n + c14_n * pow2 32 + c15_n * pow2 (2 * 32) + c8_n * pow2 (3* 32) + c9_n * pow2 (4 * 32) + c10_n * pow2 (5 * 32) + c12_n * pow2 (7 * 32)) % prime} ->
+  s8: int {s8 = (c14_n + c15_n * pow2 32 + c9_n * pow2 (3 * 32) + c10_n * pow2 (4* 32) + c11_n * pow2 (5 * 32) + c13_n * pow2 (7 * 32)) % prime} -> 
+  n: int {n = (s0 + 2 * s1 + 2 * s2 + s3 + s4 - s5 - s6 - s7 - s8) % prime} -> 
+Lemma (n % prime == (c0_n + c1_n * pow2 32 + c2_n * pow2 (2 * 32) + c3_n * pow2 (3 * 32) + c4_n * pow2 (4 * 32) + c5_n * pow2 (5 * 32) + c6_n * pow2 (6 * 32) + c7_n * pow2 (7 * 32) + c8_n * pow2 256 + c9_n * pow2 288 + c10_n * pow2 (10 * 32)  + c11_n * pow2 (11 * 32) + c12_n * pow2 (12 * 32) + c13_n* pow2 (13 * 32) + c14_n * pow2 (14 * 32) + c15_n * pow2 (15 * 32)) % prime)
+
+
+val solinas_reduction_upload0: c0: uint32 -> c1: uint32 -> c2: uint32 -> c3: uint32 -> c4: uint32 -> c5: uint32 -> 
+  c6: uint32 -> c7: uint32 -> c8: uint32 -> c9: uint32 -> c10: uint32 -> c11: uint32 -> c12: uint32 -> c13: uint32 -> 
+  c14: uint32 -> c15: uint32 -> tempBuffer: lbuffer uint64 (size 36) -> redBuffer: felem ->
+    Stack unit 
+      (fun h -> live h tempBuffer /\ live h redBuffer /\ disjoint redBuffer tempBuffer)
+      (fun h0 _ h1 -> modifies2 tempBuffer redBuffer h0 h1 /\
+	(
+	  let t0 = felem_seq_as_nat (as_seq h1 (gsub tempBuffer (size 0) (size 4))) in 
+	  let t1 = felem_seq_as_nat (as_seq h1 (gsub tempBuffer (size 4) (size 4))) in 
+	  let t2 = felem_seq_as_nat (as_seq h1 (gsub tempBuffer (size 8) (size 4))) in 
+	  let t3 = felem_seq_as_nat (as_seq h1 (gsub tempBuffer (size 12) (size 4))) in 
+	  let t4 = felem_seq_as_nat (as_seq h1 (gsub tempBuffer (size 16) (size 4))) in 
+	  let t5 = felem_seq_as_nat (as_seq h1 (gsub tempBuffer (size 20) (size 4))) in 
+ 	  t0 == (uint_v c0 + uint_v c1 * pow2 (1 * 32) + uint_v c2 * pow2 (2 * 32) + uint_v c3 * pow2 (3 * 32) + uint_v c4 * pow2 (4 * 32) + uint_v c5 * pow2 (5 * 32) + uint_v  c6 * pow2 (6 * 32) +  uint_v c7 * pow2 (7 * 32)) % prime /\
+	  t1 == (uint_v c11 * pow2 (3 * 32) + uint_v c12 * pow2 (4 * 32) + uint_v c13 * pow2 (5 * 32) + 
+	   uint_v c14 * pow2 (6 * 32) + uint_v c15 * pow2 (7 * 32)) % prime /\
+	  t2 == (uint_v c12 * pow2 (3 * 32) + uint_v c13 * pow2 (4 * 32) +  uint_v c14 * pow2 (5 * 32) + uint_v c15 * pow2 (6 * 32)) % prime  /\
+	  t3 == (uint_v c8 + uint_v c9 * pow2 32 + uint_v c10 * pow2 (2 * 32) + uint_v c14 * pow2 (6 * 32) + uint_v c15 * pow2 (7 * 32)) % prime /\
+	  t4 == (uint_v c9 + uint_v c10 * pow2 32 + uint_v c11 * pow2 (2 * 32) + uint_v c13 * pow2 (3 * 32) + uint_v c14 * pow2 (4 * 32) + uint_v c15 * pow2 (5 * 32) + uint_v c13 * pow2 (6 * 32) + uint_v c8 * pow2 (7 * 32)) % prime /\
+	  t5 == (uint_v c11 + uint_v c12 * pow2 32 + uint_v c13 * pow2 (2 * 32) + uint_v c8 * pow2 (6 * 32) + uint_v c10 * pow2 (7 * 32)) % prime
+      
+      )
+)
+
+let solinas_reduction_upload0 c0 c1 c2 c3 c4 c5 c6 c7 c8 c9 c10 c11 c12 c13 c14 c15 tempBuffer redBuffer = 
+    let t0 = sub tempBuffer (size 0) (size 4) in
+    let t1 = sub tempBuffer (size 4) (size 4) in 
+    let t2 = sub tempBuffer (size 8) (size 4) in 
+    let t3 = sub tempBuffer (size 12) (size 4) in 
+    let t4 = sub tempBuffer (size 16) (size 4) in 
+    let t5 = sub tempBuffer (size 20) (size 4) in 
+  upl_zer_buffer c0 c1 c2 c3 c4 c5 c6 c7 redBuffer t0; 
+  upl_fir_buffer c11 c12 c13 c14 c15 redBuffer t1;
+  upl_sec_buffer c12 c13 c14 c15 redBuffer t2; 
+  upl_thi_buffer c8 c9 c10 c14 c15 redBuffer  t3;
+  upl_for_buffer c8 c9 c10 c11 c13 c14 c15 redBuffer t4;
+  upl_fif_buffer c8 c10 c11 c12 c13 redBuffer  t5
+
+val solinas_reduction_upload: c0: uint32 -> c1: uint32 -> c2: uint32 -> c3: uint32 -> c4: uint32 -> c5: uint32 -> 
+  c6: uint32 -> c7: uint32 -> c8: uint32 -> c9: uint32 -> c10: uint32 -> c11: uint32 -> c12: uint32 -> c13: uint32 -> 
+  c14: uint32 -> c15: uint32 -> tempBuffer: lbuffer uint64 (size 36) -> 
+  Stack unit
+    (requires fun h -> live h tempBuffer)
+    (ensures fun h0 _ h1 -> modifies1 tempBuffer h0 h1 /\ 
+	(
+	  let t0 = felem_seq_as_nat (as_seq h1 (gsub tempBuffer (size 0) (size 4))) in 
+	  let t1 = felem_seq_as_nat (as_seq h1 (gsub tempBuffer (size 4) (size 4))) in 
+	  let t2 = felem_seq_as_nat (as_seq h1 (gsub tempBuffer (size 8) (size 4))) in 
+	  let t3 = felem_seq_as_nat (as_seq h1 (gsub tempBuffer (size 12) (size 4))) in 
+	  let t4 = felem_seq_as_nat (as_seq h1 (gsub tempBuffer (size 16) (size 4))) in 
+	  let t5 = felem_seq_as_nat (as_seq h1 (gsub tempBuffer (size 20) (size 4))) in 
+	  let t6 = felem_seq_as_nat (as_seq h1 (gsub tempBuffer (size 24) (size 4))) in 
+	  let t7 = felem_seq_as_nat (as_seq h1 (gsub tempBuffer (size 28) (size 4))) in 
+	  let t8 = felem_seq_as_nat (as_seq h1 (gsub tempBuffer (size 32) (size 4))) in 
+ 	  t0 == (uint_v c0 + uint_v c1 * pow2 (1 * 32) + uint_v c2 * pow2 (2 * 32) + uint_v c3 * pow2 (3 * 32) + uint_v c4 * pow2 (4 * 32) + uint_v c5 * pow2 (5 * 32) + uint_v  c6 * pow2 (6 * 32) +  uint_v c7 * pow2 (7 * 32)) % prime /\
+	  t1 == (uint_v c11 * pow2 (3 * 32) + uint_v c12 * pow2 (4 * 32) + uint_v c13 * pow2 (5 * 32) + 
+	   uint_v c14 * pow2 (6 * 32) + uint_v c15 * pow2 (7 * 32)) % prime /\
+	  t2 == (uint_v c12 * pow2 (3 * 32) + uint_v c13 * pow2 (4 * 32) +  uint_v c14 * pow2 (5 * 32) + uint_v c15 * pow2 (6 * 32)) % prime  /\
+	  t3 == (uint_v c8 + uint_v c9 * pow2 32 + uint_v c10 * pow2 (2 * 32) + uint_v c14 * pow2 (6 * 32) + uint_v c15 * pow2 (7 * 32)) % prime /\
+	  t4 == (uint_v c9 + uint_v c10 * pow2 32 + uint_v c11 * pow2 (2 * 32) + uint_v c13 * pow2 (3 * 32) + uint_v c14 * pow2 (4 * 32) + uint_v c15 * pow2 (5 * 32) + uint_v c13 * pow2 (6 * 32) + uint_v c8 * pow2 (7 * 32)) % prime /\
+	  t5 == (uint_v c11 + uint_v c12 * pow2 32 + uint_v c13 * pow2 (2 * 32) + uint_v c8 * pow2 (6 * 32) + uint_v c10 * pow2 (7 * 32)) % prime /\
+	  t6 == (uint_v c12 + uint_v c13 * pow2 32 + uint_v c14 * pow2 (2 * 32) + uint_v c15 * pow2 (3 * 32) + uint_v c9 * pow2 (6 * 32) + uint_v c11 * pow2 (7 * 32)) % prime /\
+	  t7 == (uint_v c13 + uint_v c14 * pow2 32 + uint_v c15 * pow2 (2 * 32) +  uint_v c8 * pow2 (3 * 32) +  uint_v c9 * pow2 (4 * 32) + uint_v c10 * pow2 (5 * 32) + uint_v c12 * pow2 (7 * 32)) % prime /\
+	  t8 == (uint_v c14 + uint_v c15 * pow2 32 + uint_v c9 * pow2 (3 * 32) +  uint_v c10 * pow2 (4 * 32) + uint_v c11 * pow2 (5 * 32) + uint_v c13 * pow2 (7 * 32)) % prime
+    ))
+
+
+let solinas_reduction_upload c0 c1 c2 c3 c4 c5 c6 c7 c8 c9 c10 c11 c12 c13 c14 c15 tempBuffer  =  
+  push_frame();
+    let redBuffer = create (size 4) (u64 0) in 
+    let t6 = sub tempBuffer (size 24) (size 4) in 
+    let t7 = sub tempBuffer (size 28) (size 4) in 
+    let t8 = sub tempBuffer (size 32) (size 4) in   
+    
+    let h0 = ST.get() in 
+    solinas_reduction_upload0 c0 c1 c2 c3 c4 c5 c6 c7 c8 c9 c10 c11 c12 c13 c14 c15 tempBuffer redBuffer;
+    upl_six_buffer c9 c11 c12 c13 c14 c15 redBuffer  t6;
+    upl_sev_buffer c8 c9 c10 c12 c13 c14 c15 redBuffer t7;
+    upl_eig_buffer c9 c10 c11 c12 c13 c14 c15 redBuffer t8;
+  pop_frame()
+  
+
 val solinas_reduction_impl: i: lbuffer uint64 (size 8) -> o: lbuffer uint64 (size 4) -> 
   Stack unit
     (requires fun h -> live h i /\ live h o /\ disjoint i o)
@@ -313,8 +427,7 @@ val solinas_reduction_impl: i: lbuffer uint64 (size 8) -> o: lbuffer uint64 (siz
 
 let solinas_reduction_impl i o = 
   push_frame();
-    let tempBuffer = create (size 36) (u64 0) in 
-    let redBuffer = create (size 4) (u64 0) in 
+    let tempBuffer = create (size 44) (u64 0) in 
     let t0 = sub tempBuffer (size 0) (size 4) in
     let t1 = sub tempBuffer (size 4) (size 4) in 
     let t2 = sub tempBuffer (size 8) (size 4) in 
@@ -324,6 +437,8 @@ let solinas_reduction_impl i o =
     let t6 = sub tempBuffer (size 24) (size 4) in 
     let t7 = sub tempBuffer (size 28) (size 4) in 
     let t8 = sub tempBuffer (size 32) (size 4) in 
+    let t11 = sub tempBuffer (size 36) (size 4) in 
+    let t22 = sub tempBuffer (size 40) (size 4) in 
 
     let i0 = i.(size 0) in 
     let i1 = i.(size 1) in 
@@ -359,20 +474,30 @@ let solinas_reduction_impl i o =
   upl_fif_buffer c8 c10 c11 c12 c13 redBuffer  t5;
   upl_six_buffer c9 c11 c12 c13 c14 c15 redBuffer  t6;
   upl_sev_buffer c8 c9 c10 c12 c13 c14 c15 redBuffer t7;
-  upl_eig_buffer c9 c10 c11 c12 c13 c14 c15 redBuffer t8;
+  upl_eig_buffer c9 c10 c11 c12 c13 c14 c15 redBuffer t8; 
 
-  p256_double t2 t2; 
-  p256_double t1 t1;
-  
-  p256_add t0 t1 o;
-  p256_add t2 o o;
+  assume(LowStar.Monotonic.Buffer.all_disjoint [loc t0; loc t1; loc t2; loc t3; loc t4; loc t5; loc t6; loc t7; loc t8; loc t11; loc t22; loc o]);
+
+  p256_double t2 t22;  
+  p256_double t1 t11;
+  p256_add t0 t11 o;
+  p256_add t22 o o;
   p256_add t3 o o;
   p256_add t4 o o;
   p256_sub o t5 o;
   p256_sub o t6 o;
   p256_sub o t7 o;
   p256_sub o t8 o;
- 
+    let h1 = ST.get() in 
+
+  modulo_lemma (felem_seq_as_nat (as_seq h1 o)) prime;
+
+  reduce_brackets (felem_seq_as_nat(as_seq h1 t0)) (felem_seq_as_nat(as_seq h1 t1)) (felem_seq_as_nat(as_seq h1 t2)) (felem_seq_as_nat(as_seq h1 t3)) (felem_seq_as_nat(as_seq h1 t4)) (felem_seq_as_nat(as_seq h1 t5)) (felem_seq_as_nat(as_seq h1 t6)) (felem_seq_as_nat(as_seq h1 t7)) (felem_seq_as_nat(as_seq h1 t8));
+  solinas_reduction_mod (uint_v c0) (uint_v c1) (uint_v c2) (uint_v c3) (uint_v c4) (uint_v c5) (uint_v c6) (uint_v c7) (uint_v c8) (uint_v c9) (uint_v c10) (uint_v c11) (uint_v c12) (uint_v c13) (uint_v c14) (uint_v c15)
+  (felem_seq_as_nat (as_seq h1 t0)) (felem_seq_as_nat (as_seq h1 t1)) (felem_seq_as_nat (as_seq h1 t2)) (felem_seq_as_nat (as_seq h1 t3))  (felem_seq_as_nat(as_seq h1 t4)) (felem_seq_as_nat(as_seq h1 t5)) (felem_seq_as_nat(as_seq h1 t6)) (felem_seq_as_nat(as_seq h1 t7)) (felem_seq_as_nat(as_seq h1 t8)) (felem_seq_as_nat (as_seq h1 o));
+  
+  admit();
+
     pop_frame() 
 
   
